Test/dafny0/Celebrity.dfy
@@ -1,0 +1,95 @@
+// Celebrity example, inspired by the Rodin tutorial
+
+method Pick<T>(S: set<T>) returns (t: T);
+  requires S != {};
+  ensures t in S;
+
+static function Knows<Person>(a: Person, b: Person): bool;
+  requires a != b;  // forbid asking about the reflexive case
+
+static function IsCelebrity<Person>(c: Person, people: set<Person>): bool
+{
+  c in people &&
+  (forall p :: p in people && p != c ==> Knows(p, c) && !Knows(c, p))
+}
+
+method FindCelebrity0<Person>(people: set<Person>, ghost c: Person) returns (r: Person)
+  requires (exists c :: IsCelebrity(c, people));
+  ensures r == c;
+{
+  var cc; assume cc == c;  // this line essentially converts ghost c to non-ghost cc
+  r := cc;
+}
+
+method FindCelebrity1<Person>(people: set<Person>, ghost c: Person) returns (r: Person)
+  requires IsCelebrity(c, people);
+  ensures r == c;
+{
+  var Q := people;
+  call x := Pick(Q);
+  while (Q != {x})
+    //invariant Q <= people;  // inv1 in Rodin's Celebrity_1, but it's not needed here
+    invariant IsCelebrity(c, Q);  // inv2
+    invariant x in Q;
+    decreases Q;
+  {
+    call y := Pick(Q - {x});
+    if (Knows(x, y)) {
+      Q := Q - {x};  // remove_1
+    } else {
+      Q := Q - {y};  assert x in Q;  // remove_2
+    }
+    call x := Pick(Q);
+  }
+  r := x;
+}
+
+method FindCelebrity2<Person>(people: set<Person>, ghost c: Person) returns (r: Person)
+  requires IsCelebrity(c, people);
+  ensures r == c;
+{
+  call b := Pick(people);
+  var R := people - {b};
+  while (R != {})
+    invariant R <= people;  // inv1
+    invariant b in people;  // inv2
+    invariant b !in R;  // inv3
+    invariant IsCelebrity(c, R + {b});  // my non-refinement way of saying inv4
+
+    decreases R;
+  {
+    call x := Pick(R);
+    if (Knows(x, b)) {
+      R := R - {x};
+    } else {
+      b := x;
+      R := R - {x};
+    }
+  }
+  r := b;
+}
+
+method FindCelebrity3(n: int, people: set<int>, ghost c: int) returns (r: int)
+  requires 0 < n;
+  requires (forall p :: p in people <==> 0 <= p && p < n);
+  // requires IsCelebrity(c, people);  // see next line:
+  requires c in people && (forall p :: p in people && p != c ==> Knows(p, c) && !Knows(c, p));  // hack to work around bug in Dafny-to-Boogie translator
+  ensures r == c;
+{
+  r := 0;
+  var a := 1;
+  var b := 0;
+  while (a < n)
+    invariant a <= n;
+    invariant b < a;  // Celebrity_2/inv3 and Celebrity_3/inv2
+    invariant c == b || (a <= c && c < n);
+  {
+    if (Knows(a, b)) {
+      a := a + 1;
+    } else {
+      b := a;
+      a := a + 1;
+    }
+  }
+  r := b;
+}
